disk-betree/DiskBetree.dfy
@@ -1,12 +1,94 @@
+include "../lib/total_order.dfy"
+include "BlockCache.dfy"  
+include "../lib/sequences.dfy"
+
 abstract module DiskBetree {
   import BC : BlockCache
+  import K : Total_Order
+  import opened Sequences
+  
+  type Key = K.Element
 
-  datatype BufferEntry = Insertion(key: Key, value: Value);
+  // Users must provide a definition of EmptyValue
+  function EmptyValue<Value>() : Value
+    
+  datatype BufferEntry<Value> = Insertion(value: Value)
 
-  datatype Buffer = Buffer(imap<Key, seq<BufferEntry>>);
-  datatype Slot = Slot(child: BC.Reference, buffer: Buffer);
-  datatype Node = Node(slots: imap<Key, Slot>);
+  type Buffer<Value> = imap<Key, seq<BufferEntry<Value>>>
+  //datatype Slot = Slot(child: BC.Reference, buffer: Buffer);
+  datatype Node<Value> = Node(children: imap<Key, BC.Reference>, buffer: Buffer<Value>)
 
-  datatype Constants = Constants(bcc: BC.Constants);
-  datatype Variables = Variables(bcv: BC.Variables);
+  datatype Layer<Value> = Layer(ref: BC.Reference, node: Node<Value>, accumulatedBuffer: seq<BufferEntry>)
+  type Lookup<Value> = seq<Layer>
+
+  predicate BufferIsDefining(log: seq<BufferEntry>) {
+    && |log| > 0
+  }
+  
+  predicate BufferDefinesValue<Value>(log: seq<BufferEntry>, value: Value) {
+    && BufferIsDefining(log)
+    && log[0].value == value
+  }
+  
+  predicate WFNode(node: Node) {
+    && (forall k :: k in node.buffer)
+    && (forall k :: k !in node.children ==> BufferIsDefining(node.buffer[k]))
+  }
+
+  predicate IsSatisfyingLookup<Value>(k: Constants, s: Variables, key: Key, value: Value, lookup: Lookup) {
+    && |lookup| > 0
+    && lookup[0].ref == BC.Root(k.bcc)
+    && (forall i :: 0 <= i < |lookup| - 1 ==> key in lookup[i].node.children && lookup[i].node.children[key] == lookup[i+1].ref)
+    && (forall i :: 0 <= i < |lookup| ==> BC.Read(k.bcc, s.bcv, lookup[i].ref, lookup[i].node))
+    && (forall i :: 0 <= i < |lookup| ==> WFNode(lookup[i].node))
+    && (forall i :: 0 <= i < |lookup| ==> lookup[i].accumulatedBuffer == (if i > 0 then lookup[i-1].accumulatedBuffer else []) + lookup[i].node.buffer[key])
+    && BufferDefinesValue(Last(lookup).accumulatedBuffer, value)
+  }
+
+  function Successors(node: Node) : iset<BC.Reference>
+  {
+    iset k | k in node.children :: node.children[k]
+  }
+  
+  // Now we define the state machine
+  
+  datatype Constants = Constants(bcc: BC.Constants)
+  datatype Variables<Value> = Variables(bcv: BC.Variables<Node<Value>>)
+
+  predicate Query<Value>(k: Constants, s: Variables, s': Variables, key: Key, value: Value, lookup: Lookup) {
+    && s == s'
+    && IsSatisfyingLookup(k, s, key, value, lookup)
+  }
+
+  predicate InsertMessage<Value>(k: Constants, s: Variables, s': Variables, key: Key, value: Value, oldroot: Node) {
+    && BC.Read(k.bcc, s.bcv, BC.Root(k.bcc), oldroot)
+    && WFNode(oldroot)
+    && var newroot := Node(oldroot.children, oldroot.buffer[key := [Insertion(value)] + oldroot.buffer[key]]);
+    && WFNode(oldroot)
+    && BC.Apply(k.bcc, s.bcv, s'.bcv, BC.WriteOp(BC.Root(k.bcc), newroot, Successors(newroot)))
+  }
+
+  predicate Flush<Value>(k: Constants, s: Variables, s': Variables, parentref: BC.Reference, parent: Node, childref: BC.Reference, child: Node, newchildref: BC.Reference, sint: BC.Variables) {
+    var movedKeys := iset k | k in parent.children && parent.children[k] == childref;
+    && BC.Read(k.bcc, s.bcv, parentref, parent)
+    && BC.Read(k.bcc, s.bcv, childref, child)
+    && WFNode(parent)
+    && WFNode(child)
+    && var newbuffer := imap k :: (if k in movedKeys then parent.buffer[k] + child.buffer[k] else child.buffer[k]);
+    && var newchild := Node(child.children, newbuffer);
+    && var newparentbuffer := imap k :: (if k in movedKeys then [] else parent.buffer[k]);
+    && var newparent := Node(parent.children, newparentbuffer);
+    && var allocop := BC.AllocOp(newchild, Successors(newchild), newchildref);
+    && var writeop := BC.WriteOp(parentref, newparent, Successors(newparent));
+    && BC.Apply2(k.bcc, s.bcv, s'.bcv, allocop, writeop)
+  }
+
+  predicate Grow(k: Constants, s: Variables, s': Variables, oldroot: Node, newchildref: BC.Reference, sint: BC.Variables) {
+    && BC.Read(k.bcc, s.bcv, BC.Root(k.bcc), oldroot)
+    && var newchild := oldroot;
+    && var newroot := Node(imap k :: newchildref, imap[]);
+    && var allocop := BC.AllocOp(newchild, Successors(newchild), newchildref);
+    && var writeop := BC.WriteOp(BC.Root(k.bcc), newroot, Successors(newroot));
+    && BC.Apply2(k.bcc, s.bcv, s'.bcv, allocop, writeop)
+  }
 }
